GCD implementation beginning

GCD.dfy
@@ -44,6 +44,118 @@ predicate GreatestCommonDivisor(a: nat, b: nat, c: nat)
 	forall d: nat :: CommonDivisor(a, b, d) ==> d <= c
 }
 
+function Remainder_Definition(a: nat, b: nat): (nat, nat)
+	requires b != 0
+{
+	(a / b, a % b)
+}
+predicate Remainder_EqualsFirst(a: nat, b: nat)
+	requires b != 0
+{
+	var (q, r) := Remainder_Definition(a, b);
+	a == (q * b) + r
+}
+lemma Remainder_Forall()
+	ensures forall a, b : nat :: b != 0 ==> Remainder_EqualsFirst(a, b)
+{
+}
+lemma Remainder_Specific(a: nat, b: nat)
+	requires b != 0
+	ensures Remainder_EqualsFirst(a, b)
+{
+}
+
+function RemiandersN(a: nat, b: nat): nat
+	requires a > 0
+	decreases b
+{
+	if b == 0 then 0
+	else 1 + RemiandersN(b, a % b)
+}
+
+function RemainderK(a: nat, b: nat, k: int): nat
+	requires a > 0
+	requires -3 <= k <= RemiandersN(a, b)
+	decreases b
+{
+	if k == -3 then b
+	else if k == -2 then a
+	else if k == -1 then b
+	else if b == 0 then a
+	else RemainderK(b, a % b, k - 1)
+}
+
+lemma {:verify false} MyL(a: nat, b: nat)
+	requires a > 0 && b > 0
+	ensures RemainderK(a, b, RemiandersN(a, b)) == 0
+	ensures forall k : nat :: k < RemiandersN(a, b) ==> RemainderK(a, b, k) > 0
+{
+}
+
+lemma {:verify false} K_LessThan_N(a: nat, b: nat, k: nat)
+	requires a > 0 && b > 0
+	requires 0 <= k <= RemiandersN(a, b)
+	requires r_k_m1_neq_0: RemainderK(a, b, k - 1) != 0
+	ensures k + 1 <= RemiandersN(a, b)
+{
+}
+
+lemma {:verify false} NextRemainerK(a: nat, b: nat, k: int)
+	requires a > 0 && b > 0
+	requires 0 <= k <= RemiandersN(a, b)
+	ensures RemainderK(a, b, k - 2) % RemainderK(a, b, k - 1) == RemainderK(a, b, k)
+{
+}
+
 method ComputeGCD(a: nat, b: nat) returns (i: nat)
 	requires a > 0 && b > 0
 	ensures GreatestCommonDivisor(a, b, i)
+{
+	// k counts the iteration number (starts with 0, zero-based).
+	// r_-2 == a, r_-1 == b
+	ghost var k : nat := 0;
+	ghost var N : nat := RemiandersN(a, b);
+	ghost var r_k_m3 := RemainderK(a, b, k);
+	var r_k_m2 := a;
+	var r_k_m1 := b;
+
+	// TODO: remove when not dafny infinitely looping
+	assert false;
+
+	while (r_k_m1 != 0)
+		invariant k <= N
+		invariant r_k_m3 == RemainderK(a, b, k - 3)
+		invariant r_k_m2 == RemainderK(a, b, k - 2)
+		invariant r_k_m1 == RemainderK(a, b, k - 1)
+		// invariant exists q_k : nat :: r_k_m3 == q_k*r_k_m2 + r_k_m1
+		decreases r_k_m1
+	{
+		K_LessThan_N(a, b, k);
+		NextRemainerK(a, b, k);
+		assert k + 1 <= N;
+		assert r_k_m2 == RemainderK(a, b, (k + 1) - 3);
+		assert r_k_m1 == RemainderK(a, b, (k + 1) - 2);
+		assert r_k_m2 % r_k_m1 == RemainderK(a, b, (k + 1) - 1);
+
+		r_k_m1, r_k_m2, r_k_m3 := r_k_m2 % r_k_m1, r_k_m1, r_k_m2;
+
+		assert k + 1 <= N;
+		assert r_k_m3 == RemainderK(a, b, (k + 1) - 3);
+		assert r_k_m2 == RemainderK(a, b, (k + 1) - 2);
+		assert r_k_m1 == RemainderK(a, b, (k + 1) - 1);
+
+		k := k + 1;
+		
+		assert k <= N;
+		assert r_k_m3 == RemainderK(a, b, k - 3);
+		assert r_k_m2 == RemainderK(a, b, k - 2);
+		assert r_k_m1 == RemainderK(a, b, k - 1);
+	}
+
+	// assert k == N;
+	// assert r_k_m3 == RemainderK(a, b, N - 3) && r_k_m2 == RemainderK(a, b, N - 2) && r_k_m1 == RemainderK(a, b, N - 1);
+	// // assert exists q_k : nat :: r_k_m3 == q_k*r_k_m2 + r_k_m1;
+	// assert r_k_m1 == 0;
+	// assert r_k_m3 % r_k_m2 == r_k_m1 == 0;
+	i := r_k_m2;
+}
